theories/Reify/Reify.v
@@ -1,10 +1,33 @@
 Require PluginUtils.PluginUtils.
 Require Import MirrorCore.Reify.Patterns.
 Require MirrorCore.Lemma.
+Require MirrorCore.Polymorphic.
 
 Declare ML Module "reify_Lambda_plugin".
 
 Export MirrorCore.Reify.Patterns.
 
 Class Reify (T : Type) : Type :=
-  reify_scheme : Command T.
+{ reify_scheme : Command T }.
+
+Arguments reify_scheme [_] _.
+
+Ltac reify_with_class X :=
+  lazymatch goal with
+  | |- ?T =>
+    let cls := constr:(@reify_scheme T _) in
+    tryif has_evar cls
+    then fail "Failed to find reification scheme for" T
+    else let cls := eval red in cls in
+         let cls := eval red in cls in
+         let k x := exact x in
+         reify_expr cls k [[ True ]] [[ X ]]
+  end.
+
+Ltac reify_type_with_class X :=
+  let x := type of X in
+  reify_with_class x.
+
+(** These are the notations for inline reification *)
+Notation "'<<:' X ':>>'" := ltac:(reify_with_class X) (at level 0, only parsing).
+Notation "'<::' X '::>'" := ltac:(reify_type_with_class X) (at level 0, only parsing).
